Cslib/Foundations/Semantics/LTS/TraceEq.lean
@@ -19,11 +19,11 @@ Definitions and results on trace equivalence for `LTS`s.
 ## Main definitions
 
 - `LTS.traces`: the set of traces of a state.
-- `TraceEq s1 s2`: `s1` and `s2` are trace equivalent, i.e., they have the same sets of traces.
+- `TraceEq s₁ s₂`: `s₁` and `s₂` are trace equivalent, i.e., they have the same sets of traces.
 
 ## Notations
 
-- `s1 ~tr[lts] s2`: the states `s1` and `s2` are trace equivalent in `lts`.
+- `s₁ ~tr[lts] s₂`: the states `s₁` and `s₂` are trace equivalent in `lts`.
 
 ## Main statements
 
@@ -44,8 +44,8 @@ theorem traces_in {lts : LTS State Label} (h : lts.MTr s μs s') : μs ∈ lts.t
 
 /-- Two states are trace equivalent if they have the same set of traces. -/
 def TraceEq (lts₁ : LTS State₁ Label) (lts₂ : LTS State₂ Label)
-    (s1 : State₁) (s2 : State₂) :=
-  lts₁.traces s1 = lts₂.traces s2
+    (s₁ : State₁) (s₂ : State₂) :=
+  lts₁.traces s₁ = lts₂.traces s₂
 
 /--
 Notation for trace equivalence.
@@ -66,14 +66,14 @@ theorem HomTraceEq.refl (s : State) : s ~tr[lts] s := by
   simp only [TraceEq]
 
 /-- Trace equivalence is symmetric. -/
-theorem TraceEq.symm (h : s1 ~tr[lts₁,lts₂] s2) : s2 ~tr[lts₂,lts₁] s1 := by
+theorem TraceEq.symm (h : s₁ ~tr[lts₁,lts₂] s₂) : s₂ ~tr[lts₂,lts₁] s₁ := by
   simp only [TraceEq] at h
   simp only [TraceEq]
   rw [h]
 
 /-- Trace equivalence is transitive. -/
-theorem TraceEq.trans (h1 : s1 ~tr[lts₁,lts₂] s2) (h2 : s2 ~tr[lts₂,lts₃] s3) :
-    s1 ~tr[lts₁,lts₃] s3 := by
+theorem TraceEq.trans (h1 : s₁ ~tr[lts₁,lts₂] s₂) (h2 : s₂ ~tr[lts₂,lts₃] s₃) :
+    s₁ ~tr[lts₁,lts₃] s₃ := by
   simp only [TraceEq] at *
   rw [h1, h2]
 
@@ -91,12 +91,12 @@ instance : Trans (TraceEq lts₁ lts₂) (TraceEq lts₂ lts₃) (TraceEq lts₁
 theorem TraceEq.deterministic_isSimulation {lts₁ : LTS State₁ Label} {lts₂ : LTS State₂ Label}
     [hdet₁ : lts₁.Deterministic] [hdet₂ : lts₂.Deterministic] :
     IsSimulation lts₁ lts₂ (TraceEq lts₁ lts₂) := by
-  intro s1 s2 h μ s1' htr1
+  intro s₁ s₂ h μ s₁' htr1
   have hmtr1 := MTr.single lts₁ htr1
   have hin := traces_in hmtr1
   rw [h] at hin
-  obtain ⟨s2', hmtr2⟩ := hin
-  exists s2'
+  obtain ⟨s₂', hmtr2⟩ := hin
+  exists s₂'
   constructor
   · apply MTr.single_invert lts₂ _ _ _ hmtr2
   · simp only [TraceEq, traces]
@@ -106,31 +106,31 @@ theorem TraceEq.deterministic_isSimulation {lts₁ : LTS State₁ Label} {lts₂
     constructor
     case mp =>
       intro hmtr1'
-      obtain ⟨s1'', hmtr1'⟩ := hmtr1'
+      obtain ⟨s₁'', hmtr1'⟩ := hmtr1'
       have hmtr1comp := MTr.comp lts₁ hmtr1 hmtr1'
       have hin := traces_in hmtr1comp
       rw [h] at hin
       obtain ⟨s', hmtr2'⟩ := hin
       cases hmtr2'
-      case stepL s2'' htr2 hmtr2' =>
+      case stepL s₂'' htr2 hmtr2' =>
         exists s'
         have htr2' := MTr.single_invert lts₂ _ _ _ hmtr2
-        have hdets2 := hdet₂.deterministic s2 μ s2' s2'' htr2' htr2
-        rw [hdets2]
+        have hdets₂ := hdet₂.deterministic s₂ μ s₂' s₂'' htr2' htr2
+        rw [hdets₂]
         exact hmtr2'
     case mpr =>
       intro hmtr2'
-      obtain ⟨s2'', hmtr2'⟩ := hmtr2'
+      obtain ⟨s₂'', hmtr2'⟩ := hmtr2'
       have hmtr2comp := MTr.comp lts₂ hmtr2 hmtr2'
       have hin := traces_in hmtr2comp
       rw [← h] at hin
       obtain ⟨s', hmtr1'⟩ := hin
       cases hmtr1'
-      case stepL s1'' htr1 hmtr1' =>
+      case stepL s₁'' htr1 hmtr1' =>
         exists s'
         have htr1' := MTr.single_invert lts₁ _ _ _ hmtr1
-        have hdets1 := hdet₁.deterministic s1 μ s1' s1'' htr1' htr1
-        rw [hdets1]
+        have hdets₁ := hdet₁.deterministic s₁ μ s₁' s₁'' htr1' htr1
+        rw [hdets₁]
         exact hmtr1'
 
 end Cslib.LTS
